src/AncillaHeap.fst
@@ -122,6 +122,5 @@ type PairHeap_mem (i:int) (ah:AncHeap) =
 *)
 
 val elts_insert : ah:AncHeap -> i:int ->
-  Lemma (requires true)
-	(ensures  (elts (insert ah i) = ins i (elts ah)))
-let elts_insert ah i =
+  Lemma (subset (elts (insert ah i)) (ins i (elts ah)))
+let elts_insert ah i = ()
